corrected some stuff

MFES/FCULEXERCISES8.dfy
@@ -1,19 +1,17 @@
 function sumNat ( n: nat) : nat
 {
-    if n == 0 then 0 else (n*(n-1))/2
+    if n == 0 then 0 else (n*(n+1))/2
 }
 
 method sum ( n: nat ) returns ( s: nat )
-    ensures s == sumNat(n+1);
+    ensures s == sumNat(n);
 {
     s := 0;
     var i := 0;
 
     while i < n 
         invariant 0 <= i <= n;
-        invariant s >= i;
-        invariant n == 0 ==> s == 0;
-        invariant s == sumNat(i+1);
+        invariant s == sumNat(i);
         decreases n - i;
     {
         i := i + 1;
