MFES/FCULEXERCISES6.dfy
@@ -6,9 +6,7 @@ method product (m: nat , n: int ) returns ( p: int )
 
     while ( i != 0 )
         invariant 0<= i <= m;
-        invariant m == 0 || n == 0 ==> p == 0;
-        invariant m == 0 ==> i == 0;
-        invariant i < 0 && m != 0 && n != 0 ==> p == m * n; 
+        invariant p == (m - i) * n; 
         decreases i;
     {
         p := p + n ;
